Fresh key package

fstar/new/MLS.fsti
@@ -5,33 +5,29 @@
 /// modifications.
 module MLS
 
+open MLS.Result
+
 val group_id: Type0
-val participant_id: Type0
 val state: group_id -> Type0
 
+// TODO: update this to identity *and* endpoint once we switch to Draft 12
+let identity = MLS.Parser.blbytes ({min=0; max=pow2 16-1})
 let bytes = MLS.Lib.Array.array Lib.IntTypes.uint8
-let group_message = group_id & bytes
-let welcome_message = participant_id & bytes
-
 let entropy = bytes
 
-val key_package: Type0
-
-noeq
-type public_info = {
-  key_package: key_package;
-  user_id: participant_id;
-}
+let group_message = group_id & bytes
+let welcome_message = identity & bytes
 
 noeq
 type private_info = {
   private_key: bytes;
 }
 
+// Always Ed25519 for the time being.
 noeq
-type credentials = {
-  signing_key: bytes;
-  identity: string;
+type credential = {
+  signature_key: MLS.Parser.blbytes ({min=0; max=pow2 16-1});
+  identity: identity;
 }
 
 // Assume here that the directory has generated a signing key for us; that our
@@ -41,20 +37,20 @@ type credentials = {
 //   The application takes care of maintaining a mapping of e.g. hash of a key
 // package to private key to be retrieved later if we are ever to receive a
 // welcome message encoded with these credentials.
-val fresh_key_package: entropy -> credentials -> key_package & private_key:bytes
+val fresh_key_package: e:entropy { Seq.length e >= 32 } -> credential -> result (bytes & private_key:bytes)
 
 // TODO: expose a way to inject e.g. a uint32 into a group_id
 // Note that after we've created the group, we receive our freshly-assigned
 // participant id.
-val create: entropy → private_info → g:group_id -> state g & participant_id
+val create: entropy → identity:string -> private_info → g:group_id -> s:state g
 
 // Internally, a new `participant_id` is assigned to the freshly-added user.
 // Provided the server does not reject the message, the application can extend
 // its mapping from the welcome message's participant_id to the corresponding
 // username and endpoint.
-val add: #g:group_id -> state g → key_package → group_message & welcome_message
+val add: #g:group_id -> s:state g → key_package → group_message & w:welcome_message
 
-val remove: #g:group_id -> state g → participant_id → group_message
+val remove: #g:group_id -> s:state g → p:identity → group_message
 
 val update: #g:group_id -> state g → entropy → group_message
 
@@ -67,6 +63,7 @@ let key_callback = bytes -> option bytes
 
 // The application provides a callback to retrieve the private key associated to
 // a key package previously generated with `fresh_key_package`.
-val process_welcome_message: welcome_message → (lookup: key_callback) -> (g:group_id & state g)
+val process_welcome_message: w:welcome_message → (lookup: key_callback) ->
+  option (g:group_id & s:state g)
 
 val process_group_message: #g:group_id -> state g → group_message → (state g & option bytes)
